BDL.lean
@@ -6,8 +6,10 @@ import BDL.Core.Satisfaction
 import BDL.Core.Env
 import BDL.Core.Dependency
 import BDL.Core.Reactive
+import BDL.Core.Clock
 import BDL.Experiments.DeclCounterexamples
 import BDL.Experiments.SemanticTypeAlternatives
 import BDL.Experiments.RepresentationBindingAlternatives
 import BDL.Experiments.DimensionAlternatives
 import BDL.Experiments.ReactiveAlternatives
+import BDL.Experiments.ClockAlternatives
